**1.** The stability of the system can be investigated using the canonical form:

$u_{n+1} = R u_n + \tau \rho_n$

, where R is the transition operator (layer transition operator).

Then from the sufficient conditions for stability it follows that if $\lambda_i$ are the eigenvalues of the layer operator, then:

1. For |$\lambda_i$| <= 1 the system will be strictly stable.
2. For |$\lambda_i$| <= 1 + C$\tau^p$ the system will be non-strictly stable.

**2.** Let's make the substitution $t' = t + 1.5$, then we get the ordinary differential equation (ODE):

$\frac{du}{dt'} = \frac{1}{1 - u\cos(t' - 1.5)} = f(t', u), \quad 0 < t' < 2.05$
$u(0) = 0$

**3.** Let's check the stability of the difference scheme:

$u_{n+1} - u_{n-1} = \tau(f(t_n, u_n) + f(t_{n-1}, u_{n-1}))$

Let's expand $f(t_{n-1}, u_{n-1})$ and $f(t_{n}, u_{n})$ in the Taylor series at the point $(t_{n}, u_{n-1})$:

$f(t_{n-1}, u_{n-1}) = f(t_{n}, u_{n-1}) + \frac{\partial f}{\partial t} (t_{n-1} - t_n) + \frac{\partial f}{\partial u} (u_{n-1} - u_{n}) + ...$
$f(t_{n}, u_{n}) = f(t_{n}, u_{n-1}) + \frac{\partial f}{\partial u} (u_{n} - u_{n - 1}) + ...$

Substituting these expansions into the difference scheme, we get:

$u_{n+1} - u_{n-1} = \tau\left(f(t_{n}, u_{n-1}) + \frac{\partial f}{\partial t} (t_{n-1} - t_n) + \frac{\partial f}{\partial u} (u_{n-1} - u_{n}) + f(t_{n}, u_{n-1}) + \frac{\partial f}{\partial u} (u_{n} - u_{n - 1}) + ...\right)$

It is difficult to bring the three-layer scheme to the canonical form, therefore, for the eigenvalues of the transition operator, we assume:


**Derivation of the condition of non-strict stability of the three-layer difference scheme for ODE:**

$u_{n+1} = u_{n-1} + \tau(f(t_n, u_n) + f(t_{n-1}, u_{n-1}))$

**Step 1:** Let's expand $f(t_{n-1}, u_{n-1})$ and $f(t_{n}, u_{n})$ in the Taylor series at the point $(t_{n}, u_{n-1})$:

$f(t_{n-1}, u_{n-1}) = f(t_{n}, u_{n-1}) + \frac{\partial f}{\partial t} (t_{n-1} - t_n) + \frac{\partial f}{\partial u} (u_{n-1} - u_{n}) + ...$
$f(t_{n}, u_{n}) = f(t_{n}, u_{n-1}) + \frac{\partial f}{\partial u} (u_{n} - u_{n - 1}) + ...$

**Step 2:** Let's substitute these expansions into the difference scheme and get:

$u_{n+1} - u_{n-1} = \tau\left(f(t_{n}, u_{n-1}) + \frac{\partial f}{\partial t} (t_{n-1} - t_n) + \frac{\partial f}{\partial u} (u_{n-1} - u_{n}) + f(t_{n}, u_{n-1}) + \frac{\partial f}{\partial u} (u_{n} - u_{n - 1}) + ...\right)$

**Step 3:** Let's group the terms and get:

$u_{n+1} - u_{n-1} = \tau\left(2f(t_{n}, u_{n-1}) + \frac{\partial f}{\partial t} (t_{n-1} - t_n) + \frac{\partial f}{\partial u} (u_{n} - 2u_{n-1}) + ...\right)$

**Step 4:** Let's write the difference scheme in the canonical form:

$u_{n+1} = \lambda u_n + \tau \rho_n$

where $\lambda = 1 + \tau\left(\frac{\partial f}{\partial t} + \frac{\partial f}{\partial u}\right)$ and $\rho_n = 2f(t_{n}, u_{n-1})$.

**Step 5:** Let's find the eigenvalues of the transition operator:

$\lambda^2 - \tau \frac{df}{du} \lambda - (1 - \tau \frac{df}{du}) = 0$

By Vieta's theorem:

$\lambda_1 \lambda_2 = - (1 + \tau \frac{df}{du})$

$\lambda_1 + \lambda_2 = \tau \frac{df}{du}$

**Step 6:** For non-strict stability, it is necessary that the eigenvalues of the transition operator be less than one in modulus:

$|\lambda_1|, |\lambda_2| < 1$

**Step 7:** Using Vieta's theorem, we get the condition of non-strict stability:

$|\frac{df}{du}| < \frac{1}{\tau}$

**In our case:**

$f(t', u) = \frac{1}{1 - u\cos(t' - 1.5)}$

$\frac{df}{du} = \frac{\cos(t' - 1.5)}{(1 - u\cos(t' - 1.5))^2}$

**Therefore, the condition of non-strict stability for the three-layer difference scheme for ODE:**

$|\frac{\cos(t' - 1.5)}{(1 - u\cos(t' - 1.5))^2}| < \frac{1}{\tau}$
